src/Narcissus/BinLib/AlignedIPChecksum.v
@@ -77,24 +77,7 @@ Definition calculate_IPChecksum {S} {sz}
   (fun v =>
      (let checksum := InternetChecksum.ByteBuffer_checksum_bound 20 v in
       (fun v idx s => SetByteAt (n := sz) 10 v 0 (wnot (split2 8 8 checksum)) ) >>
-      (fun v idx s => SetByteAt (n := sz) 11 v 0 (wnot (split1 8 8 checksum)))) v)%AlignedEncodeM.
-
-  Lemma CorrectAlignedEncoderForIPChecksumThenC
-        {S}
-        (format_A format_B : FormatM S ByteString)
-        (encode_A : forall sz, AlignedEncodeM sz)
-        (encode_B : forall sz, AlignedEncodeM sz)
-        (encoder_B_OK : CorrectAlignedEncoder format_B encode_B)
-        (encoder_A_OK : CorrectAlignedEncoder format_A encode_A)
-    : CorrectAlignedEncoder
-        (format_B ThenChecksum IPChecksum_Valid OfSize 16 ThenCarryOn format_A)
-        (fun sz => encode_B sz >>
-                   (fun v idx s => SetCurrentByte v idx (wzero 8)) >>
-                   (fun v idx s => SetCurrentByte v idx (wzero 8)) >>
-                   encode_A sz >>
-                   calculate_IPChecksum)% AlignedEncodeM.
-  Proof.
-  Admitted.
+                                                                                (fun v idx s => SetByteAt (n := sz) 11 v 0 (wnot (split1 8 8 checksum)))) v)%AlignedEncodeM.
 
 Lemma CorrectAlignedDecoderForIPChecksumThenC {A}
       predicate
@@ -126,8 +109,8 @@ Definition Pseudo_Checksum_Valid (* FIXME payload should be after src, dest *)
            (n : nat)
            (b : ByteString)
   := onesComplement (wzero 8 :: protoCode ::
-                                      (ByteString2ListOfChar (96 + n) b)
-                                      ++ to_list srcAddr ++ to_list destAddr ++ to_list (splitLength udpLength))%list
+                           (ByteString2ListOfChar (96 + n) b)
+                           ++ to_list srcAddr ++ to_list destAddr ++ to_list (splitLength udpLength))%list
      = wones 16.
 
 Import VectorNotations.
@@ -139,7 +122,7 @@ Definition pseudoHeader_checksum
            (protoCode : word 8)
            {sz} (packet: ByteBuffer.t sz) :=
   InternetChecksum.ByteBuffer_checksum_bound (12 + wordToNat udpLength)
-    (srcAddr ++ destAddr ++ [wzero 8; protoCode] ++ (splitLength udpLength) ++ packet).
+                                             (srcAddr ++ destAddr ++ [wzero 8; protoCode] ++ (splitLength udpLength) ++ packet).
 
 Infix "^1+" := (InternetChecksum.OneC_plus) (at level 50, left associativity).
 
@@ -152,10 +135,10 @@ Definition pseudoHeader_checksum'
            (protoCode : word 8)
            {sz} (packet: ByteBuffer.t sz) :=
   ByteBuffer_checksum srcAddr ^1+
-  ByteBuffer_checksum destAddr ^1+
-  zext protoCode 8 ^1+
-  udpLength ^1+
-  InternetChecksum.ByteBuffer_checksum_bound (wordToNat udpLength) packet.
+                               ByteBuffer_checksum destAddr ^1+
+                                                             zext protoCode 8 ^1+
+                                                                               udpLength ^1+
+                                                                                          InternetChecksum.ByteBuffer_checksum_bound (wordToNat udpLength) packet.
 
 Lemma OneC_plus_wzero_l :
   forall w, OneC_plus (wzero 16) w = w.
@@ -218,10 +201,10 @@ Ltac explode_vector :=
 
 Lemma pseudoHeader_checksum'_ok :
   forall (srcAddr : Vector.t (word 8) 4)
-    (destAddr : Vector.t (word 8) 4)
-    (udpLength : word 16)
-    (protoCode : word 8)
-    {sz} (packet: ByteBuffer.t sz),
+         (destAddr : Vector.t (word 8) 4)
+         (udpLength : word 16)
+         (protoCode : word 8)
+         {sz} (packet: ByteBuffer.t sz),
     pseudoHeader_checksum srcAddr destAddr udpLength protoCode packet =
     pseudoHeader_checksum' srcAddr destAddr udpLength protoCode packet.
 Proof.
@@ -233,7 +216,7 @@ Proof.
   simpl in *.
   unfold ByteBuffer_checksum, InternetChecksum.ByteBuffer_checksum_bound, add_w16_into_checksum,
   add_bytes_into_checksum, ByteBuffer_fold_left16, ByteBuffer_fold_left_pair.
-    fold @ByteBuffer_fold_left_pair.
+  fold @ByteBuffer_fold_left_pair.
   setoid_rewrite Buffer_fold_left16_acc_oneC_plus.
   rewrite combine_split.
   rewrite !OneC_plus_wzero_r, !OneC_plus_wzero_l, OneC_plus_comm.
@@ -252,7 +235,7 @@ Definition calculate_PseudoChecksum {S} {sz}
   (fun v idx s =>
      (let checksum := pseudoHeader_checksum' srcAddr destAddr udpLength protoCode v in
       (fun v idx s => SetByteAt (n := sz) idx' v 0 (wnot (split2 8 8 checksum)) ) >>
-      (fun v idx s => SetByteAt (n := sz) (1 + idx') v 0 (wnot (split1 8 8 checksum)))) v idx s)%AlignedEncodeM.
+                                                                                  (fun v idx s => SetByteAt (n := sz) (1 + idx') v 0 (wnot (split1 8 8 checksum)))) v idx s)%AlignedEncodeM.
 
 Lemma CorrectAlignedEncoderForPseudoChecksumThenC
       {S}
@@ -280,6 +263,86 @@ Proof.
 Defined.
 
 Import VectorNotations.
+
+Lemma compose_PseudoChecksum_format_correct {A}
+      (srcAddr : Vector.t (word 8) 4)
+      (destAddr : Vector.t (word 8) 4)
+      (udpLength : word 16)
+      protoCode
+      (predicate : A -> Prop)
+      (P : CacheDecode -> Prop)
+      (P_inv : (CacheDecode -> Prop) -> Prop)
+      (format_A format_B : FormatM A ByteString)
+      (formated_measure : _ -> nat)
+      (len_format_A : A -> nat)
+      (len_format_A_OK : forall a' b ctx ctx',
+          computes_to (format_A a' ctx) (b, ctx')
+          -> length_ByteString b = len_format_A a')
+      (len_format_B : A -> nat)
+      (len_format_B_OK : forall a' b ctx ctx',
+          computes_to (format_B a' ctx) (b, ctx')
+          -> length_ByteString b = len_format_B a')
+  : cache_inv_Property P P_inv ->
+    (forall a, NPeano.modulo (len_format_A a) 8 = 0)
+      -> (forall a, NPeano.modulo (len_format_B a) 8 = 0)
+      -> (forall (a : A) (ctx ctx' ctx'' : CacheFormat) c (b b'' ext : _),
+             format_A a ctx ↝ (b, ctx') ->
+             format_B a ctx' ↝ (b'', ctx'') ->
+             predicate a ->
+             len_format_A a + len_format_B a + 16 =
+             formated_measure (mappend (mappend b (mappend (format_checksum _ _ _ 16 c) b'')) ext)) ->
+      forall decodeA : _ -> CacheDecode -> option (A * _ * CacheDecode),
+        (cache_inv_Property P P_inv ->
+         CorrectDecoder monoid predicate (fun _ _ => True) (format_A ++ format_unused_word 16 ++ format_B)%format decodeA P) ->
+        CorrectDecoder monoid predicate (fun _ _ => True)
+                       (format_A ThenChecksum (Pseudo_Checksum_Valid srcAddr destAddr udpLength protoCode) OfSize 16 ThenCarryOn format_B)
+                       (fun (v : ByteString) (env : CacheDecode) =>
+                          if weq (onesComplement (wzero 8 :: protoCode ::
+                           (ByteString2ListOfChar (96 + (formated_measure v)) v)
+                           ++ to_list srcAddr ++ to_list destAddr ++ to_list (splitLength udpLength))%list) (wones 16)
+                          then
+                            decodeA v env
+                          else None) P.
+Proof.
+  intros.
+  Opaque CorrectDecoder.
+  (*eapply composeChecksum_format_correct; eauto.
+  - intros; rewrite !mappend_measure.
+    simpl; rewrite (H0 _ _ _ _ H6).
+    simpl; rewrite (H1 _ _ _ _ H7).
+    erewrite <- H4; eauto; try omega.
+    unfold format_checksum.
+    rewrite length_encode_word'.
+    simpl; omega.
+  - unfold IPChecksum_Valid in *; intros; simpl.
+    rewrite ByteString2ListOfChar_Over.
+    * rewrite ByteString2ListOfChar_Over in H9.
+      eauto.
+      simpl.
+      apply H0 in H7.
+      pose proof (H2 data).
+      rewrite <- H7 in H10.
+      rewrite !ByteString_enqueue_ByteString_padding_eq.
+      rewrite padding_eq_mod_8, H10.
+      pose proof (H3 data).
+      unfold format_checksum.
+      rewrite encode_word'_padding.
+      rewrite <- (H1 _ _ _ _ H8) in H11.
+      rewrite padding_eq_mod_8, H11.
+      reflexivity.
+    * rewrite !ByteString_enqueue_ByteString_padding_eq.
+      apply H0 in H7.
+      pose proof (H2 data).
+      rewrite <- H7 in H10.
+      rewrite padding_eq_mod_8, H10.
+      pose proof (H3 data).
+      unfold format_checksum.
+      rewrite encode_word'_padding.
+      rewrite <- (H1 _ _ _ _ H8) in H11.
+      rewrite padding_eq_mod_8, H11.
+      reflexivity.
+Qed. *)
+Admitted.
 
 Lemma CorrectAlignedDecoderForUDPChecksumThenC {A}
       (srcAddr : Vector.t (word 8) 4)
